SHA256/Preprocess.v
@@ -1,0 +1,65 @@
+Require Import List.
+Import ListNotations.
+
+(* Borrow from CompCert *)
+Require Import Coqlib.
+Require Import Bitvectors.
+
+Require Import AST.
+Require Import Semantics.
+Require Import Utils.
+Require Import Builtins.
+Require Import BuiltinSem.
+Require Import BuiltinSyntax.
+Require Import Values.        
+Require Import Bitstream.
+Require Import Lib.
+Require Import GlobalExtends.
+Require Import GetEachN.
+
+Require Import EvalTac.
+Require Import Eager.
+
+Require Import Prims.
+Require Import SHA256.
+
+(* TODO *)
+Definition preprocess_spec (msg : ext_val) : ext_val := eseq nil.
+
+
+Lemma preprocess_eval :
+  forall msg len,
+    has_type msg (tseq len tbit) ->
+    forall GE TE SE,
+      wf_env ge GE TE SE ->
+      forall ta1 ta2 ta3 ta4 tv1 tv2 tv3 padding emsg,
+        eager_eval_type GE TE ta1 tv1 ->
+        eager_eval_type GE TE ta2 tv2 ->
+        eager_eval_type GE TE ta3 tv3 ->
+        eager_eval_type GE TE ta4 (tvnum padding) ->
+        eager_eval_expr GE TE SE emsg (to_sval msg) ->
+        forall res,
+          res = to_sval (preprocess_spec msg) ->
+          eager_eval_expr GE TE SE (EApp (ETApp (ETApp (ETApp (ETApp (EVar preprocess) (ETyp ta1)) (ETyp ta2)) (ETyp ta3)) (ETyp ta4)) emsg) res.
+Proof.
+  intros.
+  gen_global preprocess.
+  gen_global (37,"split").
+  gen_global (34,"#").
+  inversion H. subst len msg t.
+  e. e. e. e. e. ag.
+  e. e. e. e. 
+  all: clear H7.
+
+  (* split_eval *)
+  e. e. e. e. e. ag. e. e. e. e.
+
+  use append_eval; try lv.
+  use append_eval; try lv.
+  
+  
+  
+Admitted.  
+
+
+    
